Make a verifier that can prove the sequential case of the parallel map program.

Skeletons/CSLTactics.v
@@ -50,8 +50,8 @@ Qed.
 
 Lemma Assn_imply (Res1 Res2 : assn) (P1 P2 : Prop) Env1 Env2 :
   incl Env2 Env1 ->
-  (P1 -> P2) ->
   (P1 -> (Res1 ===> Res2)) ->
+  (P1 -> P2) ->
   has_no_vars Res2 ->
   Assn Res1 P1 Env1 ===> Assn Res2 P2 Env2.
 Proof.
@@ -150,7 +150,6 @@ Proof.
 Qed.
 
 Create HintDb pure_lemma.
-Create HintDb no_vars_lemma.
 
 Ltac prove_mod_eq :=
   match goal with
@@ -168,19 +167,46 @@ Ltac prove_mod_eq :=
       end in
     match iter x with
     | (?t, ?u) => cutrewrite (x = t + u * n);
-      [rewrite Nat.mod_add; [|eauto] | ring];
-      apply Nat.mod_small; first [now eauto; nia]
+      [rewrite Nat.mod_add; [|eauto with pure_lemma] | ring];
+      apply Nat.mod_small; first [now eauto with pure_lemma | nia]
     end
   end.
+
+Create HintDb pure.
+
+Lemma firstn_length T i (arr : list T) :
+  length (firstn i arr) = if lt_dec i (length arr) then i else length arr.
+Proof.
+  revert arr; induction i; intros [|? ?]; destruct lt_dec; simpl in *; try omega.
+  rewrite IHi; destruct lt_dec; simpl in *; try omega.
+  rewrite IHi; destruct lt_dec; simpl in *; try omega.
+Qed.
+
+Lemma skipn_length T i (arr : list T) :
+  length (skipn i arr) = length arr - i.
+Proof.
+  revert arr; induction i; intros [|? ?]; simpl in *; try omega.
+  rewrite IHi; simpl in *; try omega.
+Qed.
+
+Hint Rewrite app_length firstn_length skipn_length : pure.
 
 Ltac prove_pure :=
   intros; 
   repeat match goal with
-  | [H : _ /\ _ |- _] => destruct H as (H & ?)
+  | [H : _ /\ _ |- _] => destruct H as [H ?]
   end; substs; repeat split;
   repeat match goal with
   | [H : context [Assn _ _ _]|- _] => clear H
   end;
+  repeat autorewrite with pure in *;
+  try now
+      repeat (match goal with
+       | [|- context [if ?b then _ else _]] => destruct b
+       | [H : context [if ?b then _ else _] |- _] => destruct b
+       | [|- context [match ?b with _ => _ end]] => destruct b
+       | [H : context [if ?b then _ else _] |- _] => destruct b
+       end);
   first [prove_mod_eq |now (eauto with pure_lemma) | nia].
 
 Ltac is_const v :=
@@ -199,6 +225,10 @@ Ltac simpl_to_zn v :=
     let v1 := simpl_to_zn v1 in
     let v2 := simpl_to_zn v2 in
     constr:(v1 + v2)
+  | (?v1 * ?v2)%Z =>
+    let v1 := simpl_to_zn v1 in
+    let v2 := simpl_to_zn v2 in
+    constr:(v1 * v2)
   | Zn ?v => v
   | ?v =>
     match is_const v with
@@ -249,8 +279,16 @@ Ltac append_assn P Q :=
   | emp => Q
   | (?P1 ** ?P2) => 
     let t := append_assn P2 Q in
-    constr:(P ** t)
+    constr:(P1 ** t)
   | _ => constr:(P ** Q)
+  end.
+
+Ltac remove_last_emp P :=
+  match P with
+  | (?P1 ** emp) => P1
+  | (?P1 ** ?P2) => 
+    let t := remove_last_emp P2 in
+    constr:(P1 ** t)
   end.
 
 (*
@@ -296,7 +334,7 @@ Ltac sep_auto :=
   intros ? ? ?;
   repeat autorewrite with sep in *;
   unfold sat in *; 
-  sep_cancel.
+  repeat sep_cancel.
 
 (*
   find an R in Res that contains le in its arguments, 
@@ -313,11 +351,11 @@ Ltac apply_read_rule Hle Hv Hn P Res le i :=
       assert (Hres : Res |= R ** Res') by sep_auto;
       assert (Hbnd : P -> i < length arr) by prove_pure;
       applys (>> rule_read_array Hle Hv Hres Hn Hbnd)
-    | sarray ?j ?d le ?arr _ _ =>
+    | array' le (skip ?arr ?d ?j) _ =>
       idtac "apply read rule: match sarray case.";
       assert (Hres : Res |= R ** Res') by sep_auto;
-      assert (Hbnd : P -> i < length arr /\ i mod d = j) by prove_pure;
-      applys (>> rule_read_sarray Hle Hv Hres Hn Hbnd); eauto
+      assert (Hbnd : P -> i < length arr /\ i mod d = j); [prove_pure|
+      applys (>> rule_read_sarray Hle Hv Hres Hn Hbnd); eauto with novars_lemma pure_lemma]
     end in
   let rec iter acc Res :=
     match Res with
@@ -328,21 +366,73 @@ Ltac apply_read_rule Hle Hv Hn P Res le i :=
     end in
   iter emp Res.
 
+(*
+  find an R in Res that contains le in its arguments, 
+  and prove resource and bound check condution, then apply appropriate rule
+ *)
+Ltac apply_write_rule Hle Hix He Hn P Res le i :=
+  let checkR Res' R :=
+    idtac "checkR: Res', R, le = " Res' "," R ", " le;
+    let Hres := fresh "Hres" in
+    let Hbnd := fresh "Hbnd" in
+    match R with
+    | array le ?arr _ =>
+      idtac "apply read rule: match array case.";
+      assert (Hres : Res |= R ** Res') by sep_auto;
+      assert (Hbnd : P -> i < length arr) by prove_pure;
+      applys (>> rule_write_array Hle Hix Hn Hbnd He Hres)
+    | array' le (skip ?arr ?d ?j) _ =>
+      idtac "apply read rule: match sarray case.";
+      assert (Hres : Res |= R ** Res') by sep_auto;
+      assert (Hbnd : P -> i < length arr /\ i mod d = j); [prove_pure|
+      applys (>> rule_write_sarray' Hle Hix Hres He Hn Hbnd); eauto with novars_lemma pure_lemma]
+    end in
+  let rec iter acc Res :=
+    match Res with
+    | ?R ** ?Res =>
+      first [let Res' := append_assn acc Res in 
+             idtac "append_assn: P, Q = " acc Res;
+               checkR Res' R |
+             iter (R ** acc) Res]
+    | ?R => let Res' := remove_last_emp acc in checkR Res' R
+    end in
+  iter emp Res.
+
 Ltac hoare_forward_prim :=
   lazymatch goal with
   | [|- CSL _ _ (Assn ?Res ?P ?Env) (?x ::T _ ::= [?le +o ?ix]) ?Q] =>
     let Hle := fresh "Hle" in let l := fresh "l" in
-    evar (l : loc); assert (Hle : evalLExp Env le l) by (unfold l; evalLExp); unfold l in Hle;
+    evar (l : loc); assert (Hle : evalLExp Env le l) by (unfold l; evalLExp); unfold l in *;
     let Hv := fresh "Hv" in let v := fresh "v" in
-    evar (v : val); assert (Hv : evalExp Env ix v) by (unfold v; evalLExp); unfold v in Hv;
+    evar (v : val); assert (Hv : evalExp Env ix v) by (unfold v; evalLExp); unfold v in *;
     let Hn := fresh "Hn" in let n := fresh "n" in
-    evar (n : nat); assert (Hn : v = Zn n) by (unfold v, n; solve_zn); unfold n in Hn;
+    evar (n : nat); assert (Hn : v = Zn n) by (unfold v, n; solve_zn); unfold n in *;
     let le := eval cbv in l in
     let i := eval cbv in n in
+    unfold l, v, n in *; clear l v n;
     apply_read_rule Hle Hv Hn P Res le i
   | [|- CSL _ _ ?P (?x ::T _ ::= [?e]) ?Q] =>
     idtac "hoare_forward_prim: match read case";
     eapply rule_read; [evalExp | find_res | ]
+  | [|- CSL _ _ (Assn ?Res ?P ?Env) ([?le +o ?ix] ::= ?e) ?Q] =>
+    idtac "hoare_forward_prim: match write array case";
+    let Hle := fresh "Hle" in let l := fresh "l" in
+    evar (l : loc); assert (Hle : evalLExp Env le l) by (unfold l; evalLExp); unfold l in *;
+
+    let Hix := fresh "Hix" in let i := fresh "i" in
+    evar (i : val); assert (Hix : evalExp Env ix i) by (unfold i; evalExp); unfold i in *;
+
+    let He := fresh "He" in let v := fresh "v" in
+    evar (v : val); assert (He : evalExp Env e v) by (unfold v; evalExp); unfold v in *;
+
+    let Hn := fresh "Hn" in let n := fresh "n" in
+    evar (n : nat); assert (Hn : i = Zn n) by (unfold i, n; solve_zn); unfold n in *;
+    
+    let l' := eval cbv in l in
+    let n' := eval cbv in n in
+    unfold l, i, v, n in *; clear l i v n;
+      
+    apply_write_rule Hle Hix He Hn P Res l' n'
   | [|- CSL _ _ ?P (?x ::T _ ::= ?e) ?Q] =>
     idtac "hoare_forward_prim: match assign case";
     eapply rule_assign; evalExp
@@ -368,32 +458,32 @@ Ltac hoare_forward :=
       first [is_evar Q; hoare_forward_prim; idtac "ok" |
              idtac "hoare_forward: match back case";
              eapply forwardR; [hoare_forward_prim|]];
-      idtac "ok"
+      simpl_env
   end.
 
-Ltac fold_sat :=
-  match goal with
-  | [|- ?P ?s ?h] =>
-    lazymatch type of s with
-    | stack => cutrewrite (P s h = sat s h P); [|reflexivity]
-    end
-  | _ => idtac
+Ltac des_conj H :=
+  repeat match type of H with
+  | _ /\ _ => 
+    let H1 := fresh "H" in
+    let H2 := fresh "H" in
+    destruct H as [H1 H2]; 
+      des_conj H1; des_conj H2
   end.
 
-Ltac fold_sat_in H :=
-  lazymatch type of H with
-  | ?P ?s ?h => 
-    lazymatch type of s with
-    | stack => cutrewrite (P s h = sat s h P) in H; [|reflexivity]
-    end
-  | _ => idtac
+Ltac des_disj H :=
+  repeat match type of H with
+  | _ \/ _ => 
+    let H1 := fresh "H" in
+    let H2 := fresh "H" in
+    destruct H as [H1 | H2]; 
+      des_disj H1; des_disj H2
   end.
 
 Ltac choose_var_vals :=
   let H := fresh in
   let e := fresh in
-  unfold incl; simpl; intros e H; 
-  repeat destruct H as [? | H]; substs; eauto 10;
+  unfold incl; simpl; intros e H;
+  des_disj H; substs; eauto 10;
   let rec tac :=
       match goal with
       | [|- ?x |-> ?v = ?x |-> ?v' \/ ?H] =>
@@ -427,28 +517,13 @@ Ltac prove_imp :=
     applys (>>Assn_imply s h H);
     [ (* proof impl. on environment *)
       choose_var_vals |
+      (* proof impl. on resource assertion *)
+      intros Hp; des_conj Hp; sep_auto |
       (* proof impl. on pure assertion *)
       let H' := fresh "H" in
-      intros H'; repeat destruct H' as (H' & ?); repeat split; substs; try prove_pure |
-      (* proof impl. on resource assertion *)
-      eauto |
+      intros H'; des_conj H'; repeat split; substs; try prove_pure |
       (* proof resource assertion does'nt have any vars *)
       eauto with novars_lemma ].
-
-Hint Resolve
-     has_no_vars_star
-     has_no_vars_mp
-     has_no_vars_emp : novars_lemma.
-
-Lemma has_no_vars_array l vs p : has_no_vars (array l vs p).
-Proof.
-  revert l; induction vs; intros l; simpl; eauto with novars_lemma.
-  apply has_no_vars_star; eauto.
-  apply has_no_vars_mp; simpl; eauto.
-  destruct l; simpl; eauto.
-Qed.
-
-Hint Resolve has_no_vars_array : novars_lemma.
 
 Module SumOf.
 
@@ -532,10 +607,12 @@ End SumOf.
 
 Module ParMap.
 
-Variable ntrd : nat.
+Variable ntrd nblk : nat.
 Hypothesis ntrd_neq_0 : ntrd <> 0.
-Hint Resolve ntrd_neq_0.
+Hypothesis nblk_neq_0 : nblk <> 0.
+Hint Resolve ntrd_neq_0 nblk_neq_0.
 Variable tid : Fin.t ntrd.
+Variable bid : Fin.t nblk.
 
 Local Notation I := (Var "I").
 Local Notation T := (Var "T").
@@ -543,47 +620,221 @@ Local Notation L := (Var "L").
 Local Notation ARR := (Var "ARR").
 Notation OUT := (Var "out").
 Notation TID := (Var "tid").
+Notation BID := (Var "bid").
 
 Definition map inv :=
-  I :T Int ::= TID ;;
+  I :T Int ::= TID +C BID *C Zn ntrd;;
   WhileI inv (I <C L) (
     T :T Int ::= [Gl ARR +o I] ;;
     [Gl OUT +o I] ::= T ;;
-    I ::= Zn ntrd +C I
+    I ::= Zn ntrd *C Zn nblk +C I
   ).
 
-Definition inv arr out varr :=
-  Ex j i vout, 
-    Assn (sarray (nf tid) ntrd (GLoc arr) varr 1%Qc 0 **
-          sarray (nf tid) ntrd (GLoc out) vout 1%Qc 0)
-         (i = j * ntrd + nf tid /\
-          i <= length varr /\
-          firstn i varr = firstn i vout)
+Notation arri a := (skip a (ntrd * nblk) (nf tid + nf bid * ntrd)).
+
+Definition inv arr out varr vout :=
+  Ex j i vs, 
+    Assn (array' (GLoc arr) (arri varr) 1%Qc **
+          array' (GLoc out) (arri vs) 1%Qc)
+         (vs = firstn i varr ++ skipn i vout /\
+          i = j * (ntrd * nblk) + (nf tid + nf bid * ntrd) /\
+          i < length varr + ntrd * nblk /\
+          length varr = length vout)
          (ARR |-> arr ::
           OUT |-> out ::
           I   |-> Zn i ::
           L   |-> (Zn (length varr)) :: nil).
 
+Lemma array'_eq ls ls' ptr p: 
+  ls = ls' -> array' ptr ls p |= array' ptr ls' p.
+Proof.
+  intros; substs; eauto.
+Qed.
+
+Lemma ok1 n m j : n + (j * n + m) = (S j) * n + m. nia. Qed.
+Lemma ok2 n m : m = 0 * n + m. nia. Qed.
+Lemma tid_bid : nf tid + nf bid * ntrd < ntrd * nblk.
+Proof.
+  pose proof ntrd_neq_0; pose proof nblk_neq_0.
+  assert (nf tid < ntrd) by eauto.
+  assert (nf bid < nblk) by eauto.
+  forwards*: (id_lt_nt_gr H1 H2).
+  lia.
+Qed.
+Lemma ntrd_nblk_neq_0 : ntrd * nblk <> 0. pose ntrd_neq_0; pose nblk_neq_0; nia. Qed.
+
+Hint Resolve ok1 ok2 tid_bid ntrd_nblk_neq_0 : pure_lemma.
+
+Lemma nth_app (T : Type) i ls1 ls2 (v : T) :
+  nth i (ls1 ++ ls2) v = if lt_dec i (length ls1) then nth i ls1 v else nth (i - length ls1) ls2 v.
+Proof.
+  revert i; induction ls1; simpl; eauto.
+  intros [|i]; simpl; eauto.
+  intros [|i]; simpl; eauto.
+  rewrite IHls1; repeat match goal with
+                | [|- context [if ?b then _ else _]] => destruct b
+                end; try omega; eauto.
+Qed.
+
+Lemma nth_firstn (T : Type) n i ls1 (v : T) :
+  nth i (firstn n ls1) v = if lt_dec i n then nth i ls1 v else v.
+Proof.
+  revert i n; induction ls1; simpl; eauto.
+  - intros [|i] [|n]; simpl; eauto.
+    destruct lt_dec; eauto.
+  - intros [|i] [|n]; simpl; eauto.
+    rewrite IHls1; repeat destruct lt_dec; try omega; eauto.
+Qed.
+
+Lemma nth_skipn (T : Type) n i ls1 (v : T) :
+  nth i (skipn n ls1) v = nth (n + i) ls1 v.
+Proof.
+  revert i n; induction ls1; eauto.
+  - intros [|i] [|n]; simpl; eauto.
+  - intros i [|n]; eauto; simpl.
+    eauto.
+Qed.        
+
+Lemma set_nth_app (T : Type) i xs ys (v : T) :
+  set_nth i (xs ++ ys) v =
+  if lt_dec i (length xs) then set_nth i xs v ++ ys
+  else xs ++ set_nth (i - length xs) ys v.
+Proof.
+  revert i; induction xs; simpl; eauto.
+  intros [|i]; simpl; eauto.
+  intros [|i]; simpl; eauto.
+  rewrite IHxs; repeat match goal with
+                | [|- context [if ?b then _ else _]] => destruct b
+                end; try omega; eauto.
+Qed.
+  
+Hint Rewrite length_set_nth ith_vals_length app_length : pure.
+Hint Rewrite nth_app nth_skip nth_set_nth nth_firstn nth_skipn : pure.
+
+Ltac t :=
+  autorewrite with pure; simpl;
+  abstract (repeat match goal with
+                   | [|- context [if ?b then _ else _]] => destruct b; substs; try lia; eauto
+                   | [H : context [if ?b then _ else _] |- _] => destruct b; substs; try lia; eauto
+                   end;
+             do 2 f_equal; lia). 
+
 Lemma map_ok BS arr out varr vout : 
   CSL BS tid 
-      (Assn (sarray (nf tid) ntrd (GLoc arr) varr 1%Qc 0 **
-             sarray (nf tid) ntrd (GLoc arr) vout 1%Qc 0)
-            True
+      (Assn (array' (GLoc arr) (arri varr) 1%Qc **
+             array' (GLoc out) (arri vout) 1%Qc)
+            (length varr = length vout)
             (TID |-> Zn (nf tid) ::
+             BID |-> Zn (nf bid) ::
              L   |-> Zn (length varr) :: 
              ARR |-> arr ::
              OUT |-> out :: nil))
-      (map (inv arr out varr))
-      (Assn (sarray (nf tid) ntrd (GLoc arr) varr 1%Qc 0 **
-             sarray (nf tid) ntrd (GLoc arr) varr 1%Qc 0)
+      (map (inv arr out varr vout))
+      (Assn (array' (GLoc arr) (arri varr) 1%Qc **
+             array' (GLoc out) (arri varr) 1%Qc)
             True
-            (TID |-> Zn (nf tid) ::
-             L   |-> Zn (length varr) ::
+            (L   |-> Zn (length varr) ::
              ARR |-> arr ::
              OUT |-> out :: nil)).
 Proof.
   unfold map, inv.
+  forwards*: (nf_lt tid).
+  forwards*: (tid_bid).
+  assert (ntrd <> 0) by eauto.
   hoare_forward.
   hoare_forward.
   hoare_forward.
+
+  (* eauto with pure_lemma. *)
+  (* do 3 lift_ex; eapply cond_prop; [evalBExp|]. *)
+  (* eapply rule_seq. *)
+  (* lazymatch goal with *)
+  (* | [|- CSL _ _ (Assn ?Res ?P ?Env) (?x ::T _ ::= [?le +o ?ix]) ?Q] => *)
+  (*   let Hle := fresh "Hle" in let l := fresh "l" in *)
+  (*   evar (l : loc); assert (Hle : evalLExp Env le l) by (unfold l; evalLExp); unfold l in *; *)
+  (*   let Hv := fresh "Hv" in let v := fresh "v" in *)
+  (*   evar (v : val); assert (Hv : evalExp Env ix v) by (unfold v; evalLExp); unfold v in *; *)
+  (*   let Hn := fresh "Hn" in let n := fresh "n" in *)
+  (*   evar (n : nat); assert (Hn : v = Zn n) by (unfold v, n; solve_zn); unfold n in *; *)
+  (*   let le := eval cbv in l in *)
+  (*   let i := eval cbv in n in *)
+  (*   unfold l, v, n in *; clear l v n; *)
+  (*   apply_read_rule Hle Hv Hn P Res le i *)
+  (* end. *)
+  (* intros;  *)
+  (* repeat match goal with *)
+  (* | [H : _ /\ _ |- _] => destruct H as [H ?] *)
+  (* end; substs; repeat split; *)
+  (* repeat match goal with *)
+  (* | [H : context [Assn _ _ _]|- _] => clear H *)
+  (* end; *)
+  (* repeat autorewrite with pure in *. *)
+  (* try now *)
+  (*     repeat (match goal with *)
+  (*             | [|- context [if ?b then _ else _]] => destruct b *)
+  (*             | [H : context [if ?b then _ else _] |- _] => destruct b *)
+  (*             | [|- context [match ?b with _ => _ end]] => destruct b *)
+  (*             | [H : context [if ?b then _ else _] |- _] => destruct b *)
+  (*             end). *)
+  (*   first [prove_mod_eq |now (eauto with pure_lemma) | lia]. *)
+  (*   first [prove_mod_eq |now (eauto with pure_lemma) | lia]. *)
+  (*   first [prove_mod_eq |now (eauto with pure_lemma) | lia]. *)
+  (* match goal with *)
+  (* | [|- ?x mod ?n = ?m] => *)
+  (*   let rec iter t := *)
+  (*     match t with *)
+  (*     | ?t + ?u => *)
+  (*       (* t = t + t' * n *) *)
+  (*       match iter t with (?t, ?t') => *)
+  (*       match iter u with (?u, ?u') => *)
+  (*       constr:(t + u, t' + u') end end *)
+  (*     | ?t * n => constr:(0, t) *)
+  (*     | n * ?t => constr:(0, t) *)
+  (*     | _ => constr:(t, 0) *)
+  (*     end in *)
+  (*   match iter x with *)
+  (*   | (?t, ?u) => cutrewrite (x = t + u * n); *)
+  (*     [rewrite Nat.mod_add; [|eauto with pure_lemma] | ring]; *)
+  (*   end *)
+  (* end. *)
   
+    
+  (*   first [prove_mod_eq |now (eauto with pure_lemma) | lia]. *)
+  hoare_forward.
+  hoare_forward.
+  prove_imp.
+  { eapply array'_eq; [|unfold sat; eauto].
+    substs.
+    revert H4 H8; clear; intros ? ?.
+    applys (>>(@eq_from_nth) (@None Z)).
+    { t. }
+    { intros i; repeat autorewrite with pure; simpl in *.
+      destruct lt_dec; [|false; lia]; intros H.
+      assert (i = j * (ntrd * nblk) + (nf tid + nf bid * ntrd) ->
+              i mod (ntrd * nblk) = nf tid + nf bid * ntrd) by (intros; substs; prove_mod_eq).
+      assert (ntrd * nblk <> 0) by eauto with pure_lemma.
+      assert (j * (ntrd * nblk) + (nf tid + nf bid * ntrd) < i < S j * (ntrd * nblk) + (nf tid + nf bid * ntrd) ->
+              i mod (ntrd * nblk) <> nf tid + nf bid * ntrd).
+      { intros; apply (mod_between j); eauto with pure_lemma. }
+      t. } }
+
+  prove_imp.
+  clear H2.
+  eapply array'_eq; [|eauto].
+  applys (>>(@eq_from_nth) (@None Z)).
+  { t. }
+  { intros.
+    repeat autorewrite with pure; simpl in *.
+    assert (i < nf tid + nf bid * ntrd -> (i mod (ntrd * nblk)) <> nf tid + nf bid * ntrd).
+    { intros; rewrite Nat.mod_small; eauto; try lia. }
+    Time t. }
+
+  prove_imp.
+  clear H2.
+  eapply array'_eq; [|unfold sat; eauto].
+  subst vs.
+  eapply (@eq_from_nth _ None).
+  { t. }
+  intros i'; repeat autorewrite with pure; simpl; intros ?.
+  t.
+Qed.
